concurrency/node-replication/InfiniteLog_Refines_NRSimple.i.dfy
@@ -9,6 +9,7 @@ abstract module InfiniteLog_Refines_NRSimple(nrifc: NRIfc) refines
   )
 {
   import opened IL = InfiniteLogSSM(nrifc)
+  import opened RequestIds
 
   predicate Inv(s: A.Variables) {
     IL.Inv(s)
@@ -26,10 +27,21 @@ abstract module InfiniteLog_Refines_NRSimple(nrifc: NRIfc) refines
   //requires A.Next(s, s', op)
   ensures Inv(s')
   {
-    //IL.NextPreservesInv(s);
+    match op {
+      case Start(rid, input) => {
+        IL.NewTicketPreservesInv(s, s', rid, input);
+      }
+      case End(rid, output) => {
+        IL.ConsumeStubPreservesInv(s, s', rid, output);
+      }
+      case InternalOp => {
+        var shard, shard', rest :| A.InternalNext(s, s', shard, shard', rest);
+        IL.InternalPreservesInv(shard, shard', rest);
+      }
+    }
   }
 
-  function I(s: A.Variables) : B.Variables
+  function I(s: A.Variables) : B.Variables // TODO fill me in
   //requires Inv(s)
 
   lemma InitRefinesInit(s: A.Variables)
@@ -37,9 +49,65 @@ abstract module InfiniteLog_Refines_NRSimple(nrifc: NRIfc) refines
   //requires Inv(s)
   ensures B.Init(I(s))
 
+  lemma NewTicket_Refines_Start(s: A.Variables, s': A.Variables,
+      rid: RequestId, input: nrifc.Input)
+  requires IL.NewTicket(s, s', rid, input)
+  requires Inv(s)
+  requires Inv(s')
+  ensures B.Next(I(s), I(s'), ifc.Start(rid, input))
+  {
+    // refine StartUpdate or StartReadonly
+  }
+
+  lemma ConsumeStub_Refines_End(s: A.Variables, s': A.Variables,
+      rid: RequestId, output: nrifc.Output)
+  requires IL.ConsumeStub(s, s', rid, output)
+  requires Inv(s)
+  requires Inv(s')
+  ensures B.Next(I(s), I(s'), ifc.End(rid, output))
+  {
+    // refine EndUpdate or EndReadonly
+  }
+
+  lemma GoToCombinerReady_Refines(s: A.Variables, s': A.Variables, nodeId: IL.NodeId)
+  requires IL.GoToCombinerReady(s, s', nodeId)
+  requires Inv(s)
+  requires Inv(s')
+  ensures B.Next(I(s), I(s'), ifc.InternalOp)
+  {
+  }
+
+  lemma Internal_Refines_Internal(s: A.Variables, s': A.Variables)
+  requires IL.Internal(s, s')
+  requires Inv(s)
+  requires Inv(s')
+  ensures B.Next(I(s), I(s'), ifc.InternalOp)
+  {
+    var step :| NextStep(s, s', step);
+    match step {
+      case GoToCombinerReady_Step(nodeId) => { GoToCombinerReady_Refines(s, s', nodeId); }
+      // ... more cases
+    }
+  }
+
   lemma NextRefinesNext(s: A.Variables, s': A.Variables, op: ifc.Op)
   //requires Inv(s)
   //requires Inv(s')
   //requires A.Next(s, s', op)
   ensures B.Next(I(s), I(s'), op)
+  {
+    match op {
+      case Start(rid, input) => {
+        NewTicket_Refines_Start(s, s', rid, input);
+      }
+      case End(rid, output) => {
+        ConsumeStub_Refines_End(s, s', rid, output);
+      }
+      case InternalOp => {
+        var shard, shard', rest :| A.InternalNext(s, s', shard, shard', rest);
+        InternalMonotonic(shard, shard', rest);
+        Internal_Refines_Internal(s, s');
+      }
+    }
+  }
 }
